src/HOL/NanoJava/OpSem.thy
@@ -9,81 +9,116 @@ header "Operational Evaluation Semantics"
 theory OpSem = State:
 
 consts
-  exec :: "(state \<times> stmt \<times> nat \<times> state) set"
+ exec :: "(state \<times> stmt       \<times> nat \<times> state) set"
+ eval :: "(state \<times> expr \<times> val \<times> nat \<times> state) set"
 syntax (xsymbols)
-  exec :: "[state,  stmt,  nat,  state] => bool" ("_ -_-_\<rightarrow> _" [98,90,99,98] 89)
+ exec :: "[state,stmt,    nat,state] => bool" ("_ -_-_\<rightarrow> _"  [98,90,   99,98] 89)
+ eval :: "[state,expr,val,nat,state] => bool" ("_ -_\<succ>_-_\<rightarrow> _"[98,95,99,99,98] 89)
 syntax
-  exec :: "[state,  stmt,  nat,  state] => bool" ("_ -_-_-> _" [98,90,99,98] 89)
+ exec :: "[state,stmt,    nat,state] => bool" ("_ -_-_-> _"  [98,90,   99,98]89)
+ eval :: "[state,expr,val,nat,state] => bool" ("_ -_>_-_-> _"[98,95,99,99,98]89)
 translations
-  "s -c-n-> s'" == "(s, c, n, s') \<in> exec"
+ "s -c  -n-> s'" == "(s, c,    n, s') \<in> exec"
+ "s -e>v-n-> s'" == "(s, e, v, n, s') \<in> eval"
 
-inductive exec intros
+inductive exec eval intros
 
   Skip: "   s -Skip-n-> s"
 
   Comp: "[| s0 -c1-n-> s1; s1 -c2-n-> s2 |] ==>
             s0 -c1;; c2-n-> s2"
 
-  Cond: "[| s -(if s<e> \<noteq> Null then c1 else c2)-n-> s' |] ==>
-            s -If(e) c1 Else c2-n-> s'"
+  Cond: "[| s0 -e>v-n-> s1; s1 -(if v\<noteq>Null then c1 else c2)-n-> s2 |] ==>
+            s0 -If(e) c1 Else c2-n-> s2"
 
-  LoopF:"   s0<e> = Null ==>
-            s0 -While(e) c-n-> s0"
-  LoopT:"[| s0<e> \<noteq> Null; s0 -c-n-> s1; s1 -While(e) c-n-> s2 |] ==>
-            s0 -While(e) c-n-> s2"
+  LoopF:"   s0<x> = Null ==>
+            s0 -While(x) c-n-> s0"
+  LoopT:"[| s0<x> \<noteq> Null; s0 -c-n-> s1; s1 -While(x) c-n-> s2 |] ==>
+            s0 -While(x) c-n-> s2"
+
+  LAcc: "   s -LAcc x>s<x>-n-> s"
+
+  LAss: "   s -e>v-n-> s' ==>
+            s -x:==e-n-> lupd(x\<mapsto>v) s'"
+
+  FAcc: "   s -e>Addr a-n-> s' ==>
+            s -e..f>get_field s' a f-n-> s'"
+
+  FAss: "[| s0 -e1>Addr a-n-> s1;  s1 -e2>v-n-> s2 |] ==>
+            s0 -e1..f:==e2-n-> upd_obj a f v s2"
 
   NewC: "   new_Addr s = Addr a ==>
-            s -x:=new C-n-> lupd(x\<mapsto>Addr a)(new_obj a C s)"
+            s -new C>Addr a-n-> new_obj a C s"
 
-  Cast: "  (case s<y> of Null => True | Addr a => obj_class s a \<preceq>C C) ==>
-            s -x:=(C)y-n-> lupd(x\<mapsto>s<y>) s"
+  Cast: "[| s -e>v-n-> s';
+            case v of Null => True | Addr a => obj_class s' a \<preceq>C C |] ==>
+            s -Cast C e>v-n-> s'"
 
-  FAcc: "   s<y> = Addr a ==>
-            s -x:=y..f-n-> lupd(x\<mapsto>get_field s a f) s"
-
-  FAss: "   s<y> = Addr a ==>
-            s -y..f:=x-n-> upd_obj a f (s<x>) s"
-
-  Call: "lupd(This\<mapsto>s<y>)(lupd(Param\<mapsto>s<p>)(init_locs C m s))-Meth C m -n-> s'==>
-            s -x:={C}y..m(p)-n-> lupd(x\<mapsto>s'<Res>)(set_locs s s')"
+  Call: "[| s0 -e1>a-n-> s1; s1 -e2>p-n-> s2; 
+            lupd(This\<mapsto>a)(lupd(Param\<mapsto>p)(init_locs C m s2)) -Meth C m-n-> s3
+     |] ==> s0 -{C}e1..m(e2)>s3<Res>-n-> set_locs s2 s3"
 
   Meth: "[| s<This> = Addr a; obj_class s a\<preceq>C C;
             s -Impl (obj_class s a) m-n-> s' |] ==>
             s -Meth C m-n-> s'"
 
-  Impl: "   s -body C m-    n-> s' ==>
+  Impl: "   s -body C m-n-> s' ==>
             s -Impl C m-Suc n-> s'"
 
-inductive_cases exec_elim_cases':
-	"s -Skip            -n-> t"
-	"s -c1;; c2         -n-> t"
-	"s -If(e) c1 Else c2-n-> t"
-	"s -While(e) c      -n-> t"
-	"s -x:=new C        -n-> t"
-	"s -x:=(C)y         -n-> t"
-	"s -x:=y..f         -n-> t"
-	"s -y..f:=x         -n-> t"
-	"s -x:={C}y..m(p)   -n-> t"
-inductive_cases Meth_elim_cases: "s -Meth C m -n-> t"
-inductive_cases Impl_elim_cases: "s -Impl C m -n-> t"
-lemmas exec_elim_cases = exec_elim_cases' Meth_elim_cases Impl_elim_cases
 
-lemma exec_mono [rule_format]: "s -c-n\<rightarrow> t \<Longrightarrow> \<forall>m. n \<le> m \<longrightarrow> s -c-m\<rightarrow> t"
-apply (erule exec.induct)
-prefer 12 (* Impl *)
+inductive_cases exec_elim_cases':
+	"s -Skip            -n\<rightarrow> t"
+	"s -c1;; c2         -n\<rightarrow> t"
+	"s -If(e) c1 Else c2-n\<rightarrow> t"
+	"s -While(x) c      -n\<rightarrow> t"
+	"s -x:==e           -n\<rightarrow> t"
+	"s -e1..f:==e2      -n\<rightarrow> t"
+inductive_cases Meth_elim_cases: "s -Meth C m-n\<rightarrow> t"
+inductive_cases Impl_elim_cases: "s -Impl C m-n\<rightarrow> t"
+lemmas exec_elim_cases = exec_elim_cases' Meth_elim_cases Impl_elim_cases
+inductive_cases eval_elim_cases:
+	"s -new C         \<succ>v-n\<rightarrow> t"
+	"s -Cast C e      \<succ>v-n\<rightarrow> t"
+	"s -LAcc x        \<succ>v-n\<rightarrow> t"
+	"s -e..f          \<succ>v-n\<rightarrow> t"
+	"s -{C}e1..m(e2)  \<succ>v-n\<rightarrow> t"
+
+lemma exec_eval_mono [rule_format]: 
+  "(s -c  -n\<rightarrow> t \<longrightarrow> (\<forall>m. n \<le> m \<longrightarrow> s -c  -m\<rightarrow> t)) \<and>
+   (s -e\<succ>v-n\<rightarrow> t \<longrightarrow> (\<forall>m. n \<le> m \<longrightarrow> s -e\<succ>v-m\<rightarrow> t))"
+apply (rule exec_eval.induct)
+prefer 14 (* Impl *)
 apply clarify
 apply (rename_tac n)
 apply (case_tac n)
-apply (blast intro:exec.intros)+
+apply  (blast intro:exec_eval.intros)+
 done
+lemmas exec_mono = exec_eval_mono [THEN conjunct1, rule_format]
+lemmas eval_mono = exec_eval_mono [THEN conjunct2, rule_format]
 
-lemma exec_max2: "\<lbrakk>s1 -c1-    n1   \<rightarrow> t1 ; s2 -c2-        n2\<rightarrow> t2\<rbrakk> \<Longrightarrow> 
-                   s1 -c1-max n1 n2\<rightarrow> t1 \<and> s2 -c2-max n1 n2\<rightarrow> t2"
+lemma exec_exec_max: "\<lbrakk>s1 -c1-    n1   \<rightarrow> t1 ; s2 -c2-       n2\<rightarrow> t2\<rbrakk> \<Longrightarrow> 
+                       s1 -c1-max n1 n2\<rightarrow> t1 \<and> s2 -c2-max n1 n2\<rightarrow> t2"
 by (fast intro: exec_mono le_maxI1 le_maxI2)
+
+lemma eval_exec_max: "\<lbrakk>s1 -c-    n1   \<rightarrow> t1 ; s2 -e\<succ>v-       n2\<rightarrow> t2\<rbrakk> \<Longrightarrow> 
+                       s1 -c-max n1 n2\<rightarrow> t1 \<and> s2 -e\<succ>v-max n1 n2\<rightarrow> t2"
+by (fast intro: eval_mono exec_mono le_maxI1 le_maxI2)
+
+lemma eval_eval_max: "\<lbrakk>s1 -e1\<succ>v1-    n1   \<rightarrow> t1 ; s2 -e2\<succ>v2-       n2\<rightarrow> t2\<rbrakk> \<Longrightarrow> 
+                       s1 -e1\<succ>v1-max n1 n2\<rightarrow> t1 \<and> s2 -e2\<succ>v2-max n1 n2\<rightarrow> t2"
+by (fast intro: eval_mono le_maxI1 le_maxI2)
+
+lemma eval_eval_exec_max: 
+ "\<lbrakk>s1 -e1\<succ>v1-n1\<rightarrow> t1; s2 -e2\<succ>v2-n2\<rightarrow> t2; s3 -c-n3\<rightarrow> t3\<rbrakk> \<Longrightarrow> 
+   s1 -e1\<succ>v1-max (max n1 n2) n3\<rightarrow> t1 \<and> 
+   s2 -e2\<succ>v2-max (max n1 n2) n3\<rightarrow> t2 \<and> 
+   s3 -c    -max (max n1 n2) n3\<rightarrow> t3"
+apply (drule (1) eval_eval_max, erule thin_rl)
+by (fast intro: exec_mono eval_mono le_maxI1 le_maxI2)
 
 lemma Impl_body_eq: "(\<lambda>t. \<exists>n. z -Impl C m-n\<rightarrow> t) = (\<lambda>t. \<exists>n. z -body C m-n\<rightarrow> t)"
 apply (rule ext)
-apply (fast elim: exec_elim_cases intro: exec.Impl)
+apply (fast elim: exec_elim_cases intro: exec_eval.Impl)
 done
 
 end
